src/Std/Data/TreeSet/Raw/Lemmas.lean
@@ -521,15 +521,21 @@ theorem mem_of_mem_union_of_not_mem_left [TransCmp cmp]
     k ∈ t₁ ∪ t₂ → ¬k ∈ t₁ → k ∈ t₂ :=
   DTreeMap.Raw.mem_of_mem_union_of_not_mem_left h₁ h₂
 
-theorem union_equiv_congr_left {t₃ : Raw α cmp} [TransCmp cmp]
+theorem Equiv.union_left {t₃ : Raw α cmp} [TransCmp cmp]
     (h₁ : t₁.WF) (h₂ : t₂.WF) (h₃ : t₃.WF) (equiv : t₁.Equiv t₂) :
     (t₁ ∪ t₃).Equiv (t₂ ∪ t₃) :=
-  ⟨TreeMap.Raw.union_equiv_congr_left h₁ h₂ h₃ equiv.1⟩
+  ⟨TreeMap.Raw.Equiv.union_left h₁ h₂ h₃ equiv.1⟩
 
-theorem union_equiv_congr_right {t₃ : Raw α cmp} [TransCmp cmp]
+theorem Equiv.union_right {t₃ : Raw α cmp} [TransCmp cmp]
     (h₁ : t₁.WF) (h₂ : t₂.WF) (h₃ : t₃.WF) (equiv : t₂.Equiv t₃) :
     (t₁ ∪ t₂).Equiv (t₁ ∪ t₃) :=
-  ⟨TreeMap.Raw.union_equiv_congr_right h₁ h₂ h₃ equiv.1⟩
+  ⟨TreeMap.Raw.Equiv.union_right h₁ h₂ h₃ equiv.1⟩
+
+theorem Equiv.union_congr {t₃ t₄ : Raw α cmp} [TransCmp cmp]
+    (h₁ : t₁.WF) (h₂ : t₂.WF) (h₃ : t₃.WF) (h₄ : t₄.WF)
+    (equiv₁ : t₁.Equiv t₃) (equiv₂ : t₂.Equiv t₄) :
+    (t₁ ∪ t₂).Equiv (t₃ ∪ t₄) :=
+  ⟨TreeMap.Raw.Equiv.union_congr h₁ h₂ h₃ h₄ equiv₁.1 equiv₂.1⟩
 
 /- get? -/
 theorem get?_union [TransCmp cmp]
